Mathbin/SetTheory/Zfc/Ordinal.lean
@@ -33,50 +33,50 @@ Further development can be found on the branch `von_neumann_v2`.
 
 universe u
 
-variable {x y z : SetCat.{u}}
+variable {x y z : ZFSet.{u}}
 
-namespace SetCat
+namespace ZFSet
 
 /-- A transitive set is one where every element is a subset. -/
-def IsTransitive (x : SetCat) : Prop :=
+def IsTransitive (x : ZFSet) : Prop :=
   ∀ y ∈ x, y ⊆ x
-#align Set.is_transitive SetCat.IsTransitive
+#align Set.is_transitive ZFSet.IsTransitive
 
 @[simp]
 theorem empty_isTransitive : IsTransitive ∅ := fun y hy => (not_mem_empty y hy).elim
-#align Set.empty_is_transitive SetCat.empty_isTransitive
+#align Set.empty_is_transitive ZFSet.empty_isTransitive
 
 theorem IsTransitive.subset_of_mem (h : x.IsTransitive) : y ∈ x → y ⊆ x :=
   h y
-#align Set.is_transitive.subset_of_mem SetCat.IsTransitive.subset_of_mem
+#align Set.is_transitive.subset_of_mem ZFSet.IsTransitive.subset_of_mem
 
-theorem isTransitive_iff_mem_trans : z.IsTransitive ↔ ∀ {x y : SetCat}, x ∈ y → y ∈ z → x ∈ z :=
+theorem isTransitive_iff_mem_trans : z.IsTransitive ↔ ∀ {x y : ZFSet}, x ∈ y → y ∈ z → x ∈ z :=
   ⟨fun h x y hx hy => h.subset_of_mem hy hx, fun H x hx y hy => H hy hx⟩
-#align Set.is_transitive_iff_mem_trans SetCat.isTransitive_iff_mem_trans
+#align Set.is_transitive_iff_mem_trans ZFSet.isTransitive_iff_mem_trans
 
 alias is_transitive_iff_mem_trans ↔ is_transitive.mem_trans _
-#align Set.is_transitive.mem_trans SetCat.IsTransitive.mem_trans
+#align Set.is_transitive.mem_trans ZFSet.IsTransitive.mem_trans
 
 protected theorem IsTransitive.inter (hx : x.IsTransitive) (hy : y.IsTransitive) :
     (x ∩ y).IsTransitive := fun z hz w hw =>
   by
   rw [mem_inter] at hz⊢
   exact ⟨hx.mem_trans hw hz.1, hy.mem_trans hw hz.2⟩
-#align Set.is_transitive.inter SetCat.IsTransitive.inter
+#align Set.is_transitive.inter ZFSet.IsTransitive.inter
 
 /- ./././Mathport/Syntax/Translate/Expr.lean:177:8: unsupported: ambiguous notation -/
-protected theorem IsTransitive.sUnion (h : x.IsTransitive) : (⋃₀ x).IsTransitive := fun y hy z hz =>
+protected theorem IsTransitive.unionₛ (h : x.IsTransitive) : (⋃₀ x).IsTransitive := fun y hy z hz =>
   by
   rcases mem_sUnion.1 hy with ⟨w, hw, hw'⟩
   exact mem_sUnion_of_mem hz (h.mem_trans hw' hw)
-#align Set.is_transitive.sUnion SetCat.IsTransitive.sUnion
+#align Set.is_transitive.sUnion ZFSet.IsTransitive.unionₛ
 
 /- ./././Mathport/Syntax/Translate/Expr.lean:177:8: unsupported: ambiguous notation -/
 theorem IsTransitive.sUnion' (H : ∀ y ∈ x, IsTransitive y) : (⋃₀ x).IsTransitive := fun y hy z hz =>
   by
   rcases mem_sUnion.1 hy with ⟨w, hw, hw'⟩
   exact mem_sUnion_of_mem ((H w hw).mem_trans hz hw') hw
-#align Set.is_transitive.sUnion' SetCat.IsTransitive.sUnion'
+#align Set.is_transitive.sUnion' ZFSet.IsTransitive.sUnion'
 
 protected theorem IsTransitive.union (hx : x.IsTransitive) (hy : y.IsTransitive) :
     (x ∪ y).IsTransitive := by
@@ -85,30 +85,30 @@ protected theorem IsTransitive.union (hx : x.IsTransitive) (hy : y.IsTransitive)
   rw [mem_pair]
   rintro (rfl | rfl)
   assumption'
-#align Set.is_transitive.union SetCat.IsTransitive.union
+#align Set.is_transitive.union ZFSet.IsTransitive.union
 
 protected theorem IsTransitive.powerset (h : x.IsTransitive) : (powerset x).IsTransitive :=
   fun y hy z hz => by
   rw [mem_powerset] at hy⊢
   exact h.subset_of_mem (hy hz)
-#align Set.is_transitive.powerset SetCat.IsTransitive.powerset
+#align Set.is_transitive.powerset ZFSet.IsTransitive.powerset
 
 /- ./././Mathport/Syntax/Translate/Expr.lean:177:8: unsupported: ambiguous notation -/
-theorem isTransitive_iff_sUnion_subset : x.IsTransitive ↔ ⋃₀ x ⊆ x :=
+theorem isTransitive_iff_unionₛ_subset : x.IsTransitive ↔ ⋃₀ x ⊆ x :=
   ⟨fun h y hy => by
     rcases mem_sUnion.1 hy with ⟨z, hz, hz'⟩
-    exact h.mem_trans hz' hz, fun H y hy z hz => H <| mem_sUnion_of_mem hz hy⟩
-#align Set.is_transitive_iff_sUnion_subset SetCat.isTransitive_iff_sUnion_subset
+    exact h.mem_trans hz' hz, fun H y hy z hz => H <| mem_unionₛ_of_mem hz hy⟩
+#align Set.is_transitive_iff_sUnion_subset ZFSet.isTransitive_iff_unionₛ_subset
 
 alias is_transitive_iff_sUnion_subset ↔ is_transitive.sUnion_subset _
-#align Set.is_transitive.sUnion_subset SetCat.IsTransitive.sUnion_subset
+#align Set.is_transitive.sUnion_subset ZFSet.IsTransitive.unionₛ_subset
 
 theorem isTransitive_iff_subset_powerset : x.IsTransitive ↔ x ⊆ powerset x :=
   ⟨fun h y hy => mem_powerset.2 <| h.subset_of_mem hy, fun H y hy z hz => mem_powerset.1 (H hy) hz⟩
-#align Set.is_transitive_iff_subset_powerset SetCat.isTransitive_iff_subset_powerset
+#align Set.is_transitive_iff_subset_powerset ZFSet.isTransitive_iff_subset_powerset
 
 alias is_transitive_iff_subset_powerset ↔ is_transitive.subset_powerset _
-#align Set.is_transitive.subset_powerset SetCat.IsTransitive.subset_powerset
+#align Set.is_transitive.subset_powerset ZFSet.IsTransitive.subset_powerset
 
-end SetCat
+end ZFSet
 
